devel/Iron/Language/SystemF2Effect/Progress.v
@@ -1,0 +1,94 @@
+
+Require Import Iron.Language.SystemF2Effect.Step.
+Require Import Iron.Language.SystemF2Effect.Store.
+Require Import Iron.Language.SystemF2Effect.TyEnv.
+Require Import Iron.Language.SystemF2Effect.TyJudge.
+Require Import Iron.Language.SystemF2Effect.KiJudge.
+
+
+(* A closed, well typed expression is either a value or can 
+   take a step in the evaluation. *)
+Theorem progress
+ :  forall se x t e s
+ ,  WfS    se s
+ -> TYPEX  nil nil se x t e
+ -> (exists v, x = XVal v) 
+ \/ (exists s' x', STEP s x s' x').
+Proof.
+ intros se x t e s HS HT.
+ gen t e.
+ induction x; intros.
+
+ Case "XVal".
+  left. 
+  exists v. trivial.
+
+ Case "XLet".
+  right.
+  inverts_type.
+  edestruct IHx1; eauto.
+  SCase "x1 value". 
+   destruct H as [v]. subst. eauto.  
+  SCase "x1 steps".
+   dests H. eauto.
+
+ Case "XApp".   
+  right.
+  inverts_type.
+  destruct v; nope.
+   SCase "v1 = VLam".
+    exists s.
+    exists (substVX 0 v0 e0). eauto.
+
+ Case "XAPP".
+  right.
+  inverts_type.
+  exists s.
+  destruct v; nope.
+   SCase "v1 = VLAM".
+    exists (substTX 0 t e). eauto.
+
+ Case "XAlloc".
+  right.
+  exists (v <: s).
+  exists (XVal (VLoc (length s))).
+  eauto.
+
+ Case "XRead".
+  right.
+  inverts_type.
+  destruct v; nope.
+  inverts_type.
+  inverts HS.
+  eapply Forall2_get_get_right in H5; eauto.
+  exists s.
+  destruct H5 as [v].
+  exists (XVal v).
+  auto.
+
+ Case "XWrite".
+  right.
+  destruct v; nope.
+  exists (update n v0 s).
+  exists (XVal (VConst CUnit)).
+  auto.
+
+ Case "XOp1".
+  destruct o.
+  SCase "OSucc".
+   inverts_type.
+   right.
+   exists s.
+   destruct v; nope.
+   destruct c; nope.
+   eauto.
+
+  SCase "OIsZero".
+   inverts_type.
+   right.
+   exists s.
+   destruct v; nope.
+   destruct c; nope.
+   eauto.
+Qed.   
+
